Merge bvm_models.lean into zfc'.lean
Cleanup

Cleanup

src/zfc'.lean
@@ -1,23 +1,448 @@
-import .fol
+import .bvm .bfol .bvm_extras .forcing .pSet_ordinal
+
+open lattice
+
+open bSet
 
 open fol
+local notation h :: t  := dvector.cons h t
+local notation `[` l:(foldr `, ` (h t, dvector.cons h t) dvector.nil `]`:0) := l
 
-/- ZFC in expanded signature -/
+local infixr ` ⟹' `:65 := lattice.imp
+local prefix `∃'` := bd_ex
+local prefix `∼` := bd_not
+local infixr ` ⊓' `:70 := bd_and
+local infixr ` ⊔' `:70 := bd_or
 
-namespace zfc'
+-- local infix ` ⟹ `:62 := bd_imp
 
-inductive ZFC'_functions : ℕ → Type
-| emptyset : ZFC'_functions 0
-| union : ZFC'_functions 1
-| pow : ZFC'_functions 1
-| pair : ZFC'_functions 2
+local infix ` ⇔' `:50 := lattice.biimp
+
+-- local infix ` ⇔ `:61 := bd_biimp
+
+universe u
+
+section ZFC'
+inductive ZFC'_rel : ℕ → Type 1
+| ε : ZFC'_rel 2
+
+inductive ZFC'_func : ℕ → Type 1
+| emptyset : ZFC'_func 0
+| pr : ZFC'_func 2
+| ω : ZFC'_func 0
+| P : ZFC'_func 1
+| Union : ZFC'_func 1
+
+def L_ZFC' : Language.{1} :=
+{ functions := ZFC'_func,
+  relations := ZFC'_rel }
+
+end ZFC'
+
+section ZFC'
+variables {β : Type 0} [nontrivial_complete_boolean_algebra β]
+
+def bSet_model_fun_map : Π {n : ℕ}, L_ZFC'.functions n → dvector (bSet β) n → bSet β :=
+begin
+  intros n S,
+    induction S,
+  from λ _, bSet.empty,
+  from λ x, by {cases x, refine bSet.pair x_x _, cases x_xs, from x_xs_x},
+  from λ _, bSet.omega,
+  from λ x, by {cases x, exact bv_powerset x_x},
+  from λ x, by {cases x, from bv_union ‹_›}
+end
+
+def bSet_model_rel_map : Π {n : ℕ}, L_ZFC'.relations n → dvector (bSet β) n → β :=
+begin
+  intros n R, induction R,
+  intro x, cases x, cases x_xs,
+  from x_x ∈ᴮ x_xs_x
+end
+
+variable (β)
+def V : bStructure L_ZFC' (β) :=
+{ carrier := (bSet β),
+  fun_map := by apply bSet_model_fun_map,
+  rel_map := by apply bSet_model_rel_map,
+  eq := bv_eq,
+  eq_refl := bv_eq_refl,
+  eq_symm := by apply bv_eq_symm,
+  eq_trans := by apply bv_eq_trans,
+  fun_congr :=
+  begin
+    intros n F, cases F,
+      {intros x y, cases x, cases y, simp},
+      tactic.rotate 1,
+      {intros x y, cases x, cases y, simp},
+      {intros x y, cases x, cases y, cases x_xs, cases y_xs,
+        change (_ ⊓ _ : β) ≤ (bv_powerset _) =ᴮ (bv_powerset _), simp,
+        tidy_context, apply bv_powerset_congr ‹_› },
+      {intros x y, cases x, cases y, cases x_xs, cases y_xs,
+        change (_ ⊓ _ : β) ≤ (bv_union _) =ᴮ (bv_union _), simp,
+        tidy_context, from bv_union_congr ‹_›},
+      {intros x y, cases x, cases y, cases x_xs, cases y_xs,
+        change (_ ⊓ (_ ⊓ _) : β) ≤ pair x_x x_xs_x =ᴮ pair y_x y_xs_x,
+        cases x_xs_xs, cases y_xs_xs, simp,
+        tidy_context, simp[*,pair_congr]}
+  end,
+  rel_congr :=
+  begin
+    intros n R, cases R, intros x y,
+    cases x, cases y, cases x_xs, cases y_xs,
+    cases x_xs_xs, cases y_xs_xs,
+    change ((_ ⊓ _) ⊓ (_ ∈ᴮ _) : β) ≤ (_ ∈ᴮ _), simp,
+    tidy_context, apply mem_congr; from ‹_›
+  end}
+
+@[simp] lemma carrier_V : ↥(V β) = bSet β := rfl
+
+@[simp]lemma V_forall {C : (V β) → β} : (⨅(x : V β), C x) = (⨅(x : bSet β), C x) := rfl
+
+@[simp]lemma V_exists {C : (V β) → β} : (⨆(x : V β), C x) = (⨆(x : bSet β), C x) := rfl
+
+@[simp]lemma V_eq {a b} : (V β).eq a b = a =ᴮ b := rfl
+
+lemma alpha_equiv₁ {C : (bSet β) → β} : (⨅(x : bSet β), C x) = ⨅(y : bSet β), C y := rfl
+lemma alpha_equiv₂ {C : (bSet β) → β} : (⨆(x : bSet β), C x) = ⨆(y : bSet β), C y := rfl
+
+def emptyset {n} : bounded_term L_ZFC' n := bd_const ZFC'_func.emptyset
+
+notation `∅'` := emptyset
+
+def omega {n} : bounded_term L_ZFC' n := bd_const ZFC'_func.ω
+
+notation `ω'` := omega
+
+def Powerset {n} : bounded_term L_ZFC' n → bounded_term L_ZFC' n := bd_app (bd_func ZFC'_func.P)
+
+notation `P'` := Powerset
+
+def mem {n} (t₁ t₂ : bounded_term L_ZFC' n) : bounded_formula L_ZFC' n :=
+@bounded_formula_of_relation L_ZFC' 2 n ZFC'_rel.ε t₁ t₂
+
+local infix ` ∈'`:100 := _root_.mem
+
+def pair' {n} (t₁ t₂ : bounded_term L_ZFC' n) : bounded_term L_ZFC' n :=
+@bounded_term_of_function L_ZFC' 2 n ZFC'_func.pr t₁ t₂
+
+def union' {n} : bounded_term L_ZFC' n → bounded_term L_ZFC' n := bd_app (bd_func ZFC'_func.Union)
+
+notation `⋃'` := union'
+
+local prefix `&'`:max := bd_var
 
 
-inductive ZFC'_relations : ℕ → Type
-| ϵ : ZFC'_relations 2
-| subset : ZFC'_relations 2
+@[simp] lemma boolean_realize_bounded_formula_mem {n} {v : dvector (V β) n}
+  (t₁ t₂ : bounded_term L_ZFC' n) :
+  boolean_realize_bounded_formula v (t₁ ∈' t₂) ([]) =
+  boolean_realize_bounded_term v t₁ ([]) ∈ᴮ boolean_realize_bounded_term v t₂ ([]) :=
+by refl
 
-def L_ZFC' : Language :=
-⟨ZFC'_functions, ZFC'_relations⟩
+@[simp] lemma boolean_realize_bounded_term_Union {n} {v : dvector (V β) n}
+  (t : bounded_term L_ZFC' n) :
+  boolean_realize_bounded_term v (⋃' t) ([]) =
+  bv_union (boolean_realize_bounded_term v t ([])) :=
+by refl
 
-end zfc'
+@[simp] lemma boolean_realize_bounded_term_Powerset {n} {v : dvector (V β) n}
+  (t : bounded_term L_ZFC' n) :
+  boolean_realize_bounded_term v (P' t) ([]) =
+  bv_powerset (boolean_realize_bounded_term v t ([])) :=
+by refl
+
+@[simp] lemma boolean_realize_bounded_term_omega {n} {v : dvector (V β) n} :
+  boolean_realize_bounded_term v ω' ([]) = bSet.omega :=
+by refl
+
+@[simp] lemma boolean_realize_bounded_term_emptyset {n} {v : dvector (V β) n} :
+  boolean_realize_bounded_term v ∅' ([]) = bSet.empty :=
+by refl
+
+@[simp]lemma boolean_realize_bounded_term_pair {n} {v : dvector (V β) n}
+  (t₁ t₂ : bounded_term L_ZFC' n) :  boolean_realize_bounded_term v (pair' t₁ t₂) ([]) =
+  pair (boolean_realize_bounded_term v t₁ ([])) (boolean_realize_bounded_term v t₂ ([])) :=
+by refl
+
+@[simp] lemma fin_0 {n : ℕ} : (0 : fin (n+1)).1 = 0 := by refl
+@[simp] lemma fin_1 {n : ℕ} : (1 : fin (n+2)).1 = 1 := by refl
+@[simp] lemma fin_2 {n : ℕ} : (2 : fin (n+3)).1 = 2 := by refl
+@[simp] lemma fin_3 {n : ℕ} : (3 : fin (n+4)).1 = 3 := by refl
+
+def axiom_of_emptyset : sentence L_ZFC' := ∀' (∼(&0 ∈' ∅'))
+
+lemma bSet_models_emptyset : ⊤ ⊩[V β] axiom_of_emptyset :=
+by {change ⊤ ≤ _, simp[axiom_of_emptyset, -top_le_iff], intro x, from empty_spec}
+
+def axiom_of_pairing : sentence L_ZFC' :=
+ ∀' ∀' ∀' ∀'(((pair' &'3 &'2 ≃pair' &'1 &'0)) ⇔ (&'3 ≃ &'1 ⊓ &'2 ≃ &'0))
+
+lemma bSet_models_pairing : ⊤ ⊩[V β] axiom_of_pairing :=
+begin
+  change ⊤ ≤ _, simp[axiom_of_pairing], intros a b x y, tidy,
+  from eq_of_eq_pair_left, from eq_of_eq_pair_right,
+  simp[pair_congr]
+end
+
+-- axiom of extensionality
+-- ∀ x y, (∀ z, (z ∈ x ↔ z ∈ y)) → x = y
+def axiom_of_extensionality : sentence L_ZFC' :=
+∀' ∀' (∀'(&'0  ∈' &'2 ⇔  &'0 ∈' &'1) ⟹ (&1 ≃ &0))
+
+lemma bSet_models_extensionality : ⊤ ⊩[V β] axiom_of_extensionality :=
+by { simp [forced_in, axiom_of_extensionality], exact bSet_axiom_of_extensionality }
+
+-- axiom of collection
+-- For every formula ϕ(x,y),
+-- ∀ u, (∀ x ∈ u, ∃ y, ϕ(x,y)) ⟹ (∃ v, ∀ z ∈ u, ∃ w ∈ v, ϕ(z,w))
+
+def axiom_of_collection (ϕ' : bounded_formula L_ZFC' 2) : sentence L_ZFC' :=
+∀' ((∀' (&'0 ∈' &'1 ⟹ ∃' ϕ'.cast1)) ⟹
+(∃' ∀'(&'0 ∈' &'2 ⟹ ∃' (&'0 ∈' &'2 ⊓ ϕ'.cast dec_trivial))))
+
+-- note: should write a lemma which says given the full congr lemma for a 2-ary formula, can extract left and right congr lemmas
+lemma bSet_models_collection (ϕ : bounded_formula L_ZFC' 2) : ⊤ ⊩[V β] axiom_of_collection ϕ :=
+begin
+  change ⊤ ≤ _, bv_intro u, simp, have := bSet_axiom_of_collection' _ _ _ u,
+  simp only [lattice.top_le_iff, bSet.mem, lattice.imp_top_iff_le, lattice.le_infi_iff] at this,
+  exact this u,
+  { intros,
+    let v₁ : ℕ → V β := λ n, nat.rec_on n x (λ _ _, z),
+    let v₂ : ℕ → V β := λ n, nat.rec_on n y (λ _ _, z),
+    have h₁ : ∀(k : ℕ) (hk : k < 2), v₁ k = dvector.nth ([x, z]) k hk,
+    { intros, cases k, refl, cases k, refl, exfalso, apply not_le_of_gt hk,
+      apply nat.succ_le_succ, apply nat.succ_le_succ, apply nat.zero_le },
+    have h₂ : ∀(k : ℕ) (hk : k < 2), v₂ k = dvector.nth ([y, z]) k hk,
+    { intros, cases k, refl, cases k, refl, exfalso, apply not_le_of_gt hk,
+      apply nat.succ_le_succ, apply nat.succ_le_succ, apply nat.zero_le },
+    rw [←boolean_realize_bounded_formula_eq h₁, ←boolean_realize_bounded_formula_eq h₂],
+    convert boolean_realize_formula_congr _ _ _ _,
+    apply le_antisymm, apply le_infi, intro n, cases n,
+    refl, simp only [v₁, v₂, bStructure.eq_refl, le_top],
+    apply infi_le _ 0 },
+  { intros,
+    let v₁ : ℕ → V β := λ n, nat.rec_on n z (λ _ _, x),
+    let v₂ : ℕ → V β := λ n, nat.rec_on n z (λ _ _, y),
+    have h₁ : ∀(k : ℕ) (hk : k < 2), v₁ k = dvector.nth ([z, x]) k hk,
+    { intros, cases k, refl, cases k, refl, exfalso, apply not_le_of_gt hk,
+      apply nat.succ_le_succ, apply nat.succ_le_succ, apply nat.zero_le },
+    have h₂ : ∀(k : ℕ) (hk : k < 2), v₂ k = dvector.nth ([z, y]) k hk,
+    { intros, cases k, refl, cases k, refl, exfalso, apply not_le_of_gt hk,
+      apply nat.succ_le_succ, apply nat.succ_le_succ, apply nat.zero_le },
+    rw [←boolean_realize_bounded_formula_eq h₁, ←boolean_realize_bounded_formula_eq h₂],
+    convert boolean_realize_formula_congr _ _ _ _,
+    apply le_antisymm, apply le_infi, intro n, cases n,
+    simp only [v₁, v₂, bStructure.eq_refl, le_top], refl,
+    apply infi_le _ 1 },
+end
+
+-- axiom of union
+-- ∀ u x, x ∈ ⋃ u ↔ ∃ y ∈ u, x ∈ y
+def axiom_of_union : sentence L_ZFC' :=
+∀' ∀' (&'0 ∈' ⋃' &'1 ⇔ (∃' (&'0 ∈' &'2 ⊓ &'1 ∈' &'0)))
+
+lemma bSet_models_union : ⊤ ⊩[V β] axiom_of_union :=
+begin
+  simp [-top_le_iff, forced_in, axiom_of_union, -lattice.le_inf_iff],
+  intros x z,
+  have := @bv_union_spec' _ _ x ⊤,
+  replace this := this z, dsimp at this,
+  bv_split, bv_split_goal
+end
+
+-- axiom of powerset
+-- ∀ u x, x ∈ P(x) ↔ ∀ y ∈ x, y ∈ u
+
+def axiom_of_powerset : sentence L_ZFC' :=
+  ∀' ∀' (&'0 ∈' P' &'1 ⇔ (∀' (&'0 ∈' &'1 ⟹ &'0 ∈' &'2)))
+
+lemma bSet_models_powerset : ⊤ ⊩[V β] axiom_of_powerset :=
+begin
+  simp [forced_in, axiom_of_powerset, -lattice.le_inf_iff, -top_le_iff],
+  intros x z, have := @bv_powerset_spec _ _ x z,
+  rw [subset_unfold'] at this,
+  apply le_inf, bv_imp_intro, exact this.mpr H, bv_imp_intro, exact this.mp H
+end
+
+-- axiom of infinity
+-- ∅ ∈ ω ∧ ∀ x ∈ ω, ∃ y ∈ ω, x ∈ y
+
+def axiom_of_infinity : sentence L_ZFC' :=
+  ∅' ∈' ω' ⊓ ∀'(&'0 ∈' ω' ⟹ ∃' (&'0 ∈' ω' ⊓' &'1 ∈' &'0))
+
+lemma bSet_models_infinity : ⊤ ⊩[V β] axiom_of_infinity :=
+begin
+  simp [forced_in, axiom_of_infinity, boolean_realize_sentence, -lattice.le_inf_iff, -top_le_iff],
+  exact bSet_axiom_of_infinity'
+end
+
+-- axiom of regularity
+-- ∀ x, x ≠ ∅ ⟹ ∃ y ∈ x, ∀ z' ∈ x, ¬ (z' ∈ y)
+
+def axiom_of_regularity : sentence L_ZFC' :=
+  ∀' (∼(&0 ≃ ∅') ⟹ (∃' (&'0 ∈' &'1 ⊓ ∀' (&'0 ∈' &'2 ⟹ ∼(&'0 ∈' &'1)))))
+
+lemma bSet_models_regularity : ⊤ ⊩[V β] axiom_of_regularity :=
+begin
+  change ⊤ ≤ _, unfold axiom_of_regularity,
+  simp[-top_le_iff], intro x,
+  bv_imp_intro,
+  apply bSet_axiom_of_regularity, convert H
+end
+
+/-- &1 ⊆ &0 ↔ ∀ z, (z ∈ &1 ⟹ z ∈ &0)-/
+def subset'' {n} (t₁ t₂ : bounded_term L_ZFC' n): bounded_formula L_ZFC' n :=
+∀' (&'0 ∈' (t₁ ↑ 1) ⟹ &'0 ∈' (t₂ ↑ 1))
+
+local infix ` ⊆'`:100 := subset''
+
+@[simp] lemma boolean_realize_bounded_formula_subset {n} {v : dvector (V β) n}
+  (t₁ t₂ : bounded_term L_ZFC' n) :
+  boolean_realize_bounded_formula v (t₁ ⊆' t₂) ([]) =
+  boolean_realize_bounded_term v t₁ ([]) ⊆ᴮ boolean_realize_bounded_term v t₂ ([]) :=
+by { simp [subset'', subset_unfold'] }
+
+def zorns_lemma : sentence L_ZFC' :=
+∀' (∼ (&'0 ≃ ∅')
+  ⟹ (∀' (&'0 ⊆' &'1 ⊓' (∀' ∀' ((&'1 ∈' &'2 ⊓' &'0 ∈' &'2) ⟹ (&'1 ⊆' &'0 ⊔' &'0 ⊆' &'1)))
+    ⟹ (⋃' &' 0 ∈' &'1)))
+    ⟹  (∃' (&'0 ∈' &'1 ⊓ ∀' (&'0 ∈' &'2 ⟹ &'1 ⊆' &'0 ⟹ &'1 ≃ &'0 ))))
+
+lemma bSet_models_Zorn : ⊤ ⊩[V β] zorns_lemma :=
+begin
+  simp [forced_in, zorns_lemma, boolean_realize_sentence, -lattice.le_inf_iff, -top_le_iff, -lattice.le_infi_iff],
+  from bSet_zorns_lemma'
+end
+
+def ZFC' : Theory L_ZFC' :=
+  {axiom_of_emptyset, axiom_of_pairing, axiom_of_extensionality,
+  axiom_of_union, axiom_of_powerset, axiom_of_infinity,
+  axiom_of_regularity, zorns_lemma} ∪ (axiom_of_collection '' (set.univ))
+
+theorem bSet_models_ZFC' : ⊤ ⊩[V β] ZFC' :=
+begin
+  change ⊤ ≤ _, bv_intro f, bv_intro H,
+  repeat{auto_cases}; try{subst H}; try {cases H},
+  from bSet_models_Zorn _,
+  from bSet_models_regularity _,
+  from bSet_models_infinity _,
+  from bSet_models_powerset _,
+  from bSet_models_union _,
+  from bSet_models_extensionality _,
+  from bSet_models_pairing _,
+  from bSet_models_emptyset _,
+  from bSet_models_collection _ ‹_›
+end
+
+/-- f is =ᴮ-extensional if for every w₁ w₂ v₁ v₂, if pair (w₁ v₁) and pair (w₂ v₂) ∈ f and
+    w₁ =ᴮ w₂, then v₁ =ᴮ v₂ -/
+def is_extensional_f : bounded_formula L_ZFC' 1 :=
+∀' ∀' ∀' ∀' ((pair' &'3 &'1 ∈' &'4 ⊓' pair' &'2 &'0 ∈' &'4
+  ⟹ (&'3 ≃ &'2 ⟹ &'1 ≃ &'0)))
+
+@[simp]lemma realize_is_extensional_f {f : V β} : boolean_realize_bounded_formula (by exact [f]) is_extensional_f dvector.nil = is_extensional f :=
+begin
+  simp[is_extensional_f, bSet.is_extensional], refl
+end
+
+def is_functional_f : bounded_formula L_ZFC' 1 :=
+∀' ((∃' (pair' &'1 &'0 ∈' &'2)) ⟹ (∃' ∀' (pair' &'2 &'0 ∈' &'3 ⟹ &'1 ≃ &'0)))
+
+@[simp]lemma realize_is_functional_f (f : V β) :  boolean_realize_bounded_formula (by exact [f]) is_functional_f dvector.nil = is_functional f :=
+begin
+  simp[is_functional_f, bSet.is_functional]
+end
+
+def is_func_f : bounded_formula L_ZFC' 1 :=
+  is_extensional_f ⊓' is_functional_f
+
+@[simp]lemma realize_is_func_f {f : V β} : begin apply boolean_realize_bounded_formula, from [f], from is_func_f, from dvector.nil end = is_func f :=
+begin
+  simp[is_func_f, bSet.is_func]
+end
+
+def is_func'_f : bounded_formula L_ZFC' 3 :=
+  (is_func_f.cast (dec_trivial)) ⊓' (∀' (&'0 ∈' &'3 ⟹ (∃' (&'0 ∈' &'3 ⊓' (pair' &'1 &'0 ∈' &'2)))))
+
+@[simp]lemma realize_is_func'_f {x y f : V β} : boolean_realize_bounded_formula (by exact [f, y, x]) is_func'_f dvector.nil = is_func' x y f :=
+begin
+  simp[is_func', is_func, is_func'_f, is_func_f]
+end
+
+def larger_than_f : bounded_formula L_ZFC' 2 :=
+∃' (is_func_f.cast (dec_trivial) ⊓
+   ∀' ( &0 ∈' &2 ⟹ (∃' (&'0 ∈' &'4 ⊓' pair' &'0 &'1 ∈' &'2))))
+
+@[simp]lemma realize_larger_than_f {x y : V β} :
+  boolean_realize_bounded_formula (by exact [y,x]) larger_than_f dvector.nil = larger_than x y :=
+begin
+  simp[larger_than, larger_than_f, is_func, is_func_f], refl
+end
+
+def is_inj_f : bounded_formula L_ZFC' 1 :=
+∀' ∀' ∀' ∀' (((pair' &'3 &'1 ∈' &'4 ⊓' pair' &'2 &'0 ∈' &'4) ⊓ &'1 ≃ &'0) ⟹ &'3 ≃ &'2)
+
+@[simp]lemma realize_is_inj_f (f : V β) :
+  boolean_realize_bounded_formula (by exact [f]) is_inj_f dvector.nil = is_inj f :=
+by {simp[is_inj_f, is_inj], refl}
+
+def injects_into_f : bounded_formula L_ZFC' 2 :=
+ ∃' (is_func'_f ⊓' is_inj_f.cast (dec_trivial)) 
+
+@[simp]lemma realize_injects_into {x y : V β} :
+  boolean_realize_bounded_formula (by exact [y,x]) injects_into_f dvector.nil = injects_into x y :=
+by {simp[injects_into_f, injects_into]}
+
+-- @[simp]lemma realize_injects_into_subst0 {y : V β} {t : bounded_term L_ZFC' 1}:
+--   -- boolean_realize_bounded_formula (by exact [boolean_realize_closed_term t])
+--   boolean_realize_bounded_formula (by exact [y]) (injects_into_f[t /0]) dvector.nil = injects_into (by exact (boolean_realize_bounded_term (by exact [y]) t dvector.nil)) y :=
+-- sorry
+
+--⨆ x, ⨆y, (ℵ₀ ≺ x) ⊓ (x ≺ y) ⊓ (y ≼ 𝒫(ℵ₀))
+
+def CH_f : sentence L_ZFC' :=
+(∀' (∀' (∼((∼(substmax_bounded_formula (larger_than_f) ω' ↑ 1) ⊓'
+  ∼larger_than_f ⊓' (injects_into_f[(Powerset omega) /0].cast1))))))
+
+lemma subst_unfold₁ : ((substmax_bounded_formula (larger_than_f) ω' ↑ 1)) =
+  ∃' ((is_func_f.cast (dec_trivial)) ⊓
+    ∀' (&0 ∈' &3 ⟹ (∃' (&'0 ∈' (ω') ⊓' pair' &'0 &'1 ∈' &'2)))) := rfl
+
+lemma subst_unfold₂ : (injects_into_f[P' omega /0]) = ∃'(((is_func_f.cast (dec_trivial) ⊓'
+  (∀' (&'0 ∈' &'2 ⟹ (∃' (&'0 ∈' (Powerset omega) ⊓' (pair' &'1 &'0 ∈' &'2))))))
+  ⊓' is_inj_f.cast (dec_trivial))) := rfl
+
+
+end ZFC'
+
+open pSet cardinal
+
+section CH_unprovable
+
+lemma neg_CH_f : ⊤ ⊩[V 𝔹] ∼CH_f :=
+begin
+  change ⊤ ≤ _, simp[-top_le_iff, CH_f], simp only [neg_infi],
+  apply bv_use (ℵ₁̌ ), apply bv_use (ℵ₂ ̌), simp[-top_le_iff],
+  refine ⟨_,ℵ₁_lt_ℵ₂,_⟩,
+  {have := ℵ₀_lt_ℵ₁, unfold larger_than at this, have := subst_unfold₁,
+  unfold substmax_bounded_formula at this, rw[this],
+  simp[-top_le_iff], simp only [neg_supr] at *, bv_intro f,
+  bv_specialize_at this (f), from this_1},
+  {have := ℵ₂_le_𝔠, rw[subst_unfold₂], simp[-top_le_iff],
+    apply bv_use (neg_CH_func), from this}
+end
+
+instance V_𝔹_nonempty : nonempty (V 𝔹) := ⟨bSet.empty⟩
+
+theorem CH_f_unprovable : ¬ (ZFC' ⊢' CH_f) :=
+begin
+  intro H,
+  suffices forces_false : ⊤ ⊩[V 𝔹] bd_falsum,
+    from absurd (nontrivial.bot_lt_top) (not_lt_of_le forces_false),
+  refine forced_absurd _ _, exact ZFC', exact CH_f, swap, apply neg_CH_f,
+  let prf_of_CH_f := sprovable_of_provable (classical.choice H),
+  have CH_f_true := boolean_soundness prf_of_CH_f (V_𝔹_nonempty),
+  convert CH_f_true, rw[inf_axioms_top_of_models (bSet_models_ZFC' _)]
+end
+
+end CH_unprovable
